thy/Rot13.thy
@@ -37,4 +37,10 @@ value[code] "map byte_to_char (run_bf (parse_instrs rot13) (map char_to_byte ''H
 lemma "let result = run_bf (parse_instrs rot13) (map char_to_byte ''Hello World!'') in
          map byte_to_char result = ''Uryyb Jbeyq!''" by eval
 
+(*Not working*)
+value "bounded_machine 20000 (parse_instrs rot13) [] (empty_tape, Buffer (map char_to_byte ''Hello World!'') read_byte [])"
+
+value "let result = run_bf_bounded 34502004 (parse_instrs rot13) (map char_to_byte ''Hello World!'') in
+         map byte_to_char result"
+
 end
